ulib/FStar.Pervasives.fst
@@ -19,8 +19,8 @@ effect Dv (a:Type) =
    as being impure but having no observable effect on the state *)
 effect EXT (a:Type) = Dv a
 
-let st_pre_h   (heap:Type) = heap -> GTot Type0
-let st_post_h' (heap:Type) (a:Type) (pre:Type) = a -> (_:heap{pre}) -> GTot Type0
+let st_pre_h   (heap:Type) = heap -> GTot prop
+let st_post_h' (heap:Type) (a:Type) (pre:prop) = a -> (_:heap{pre}) -> GTot prop
 let st_post_h  (heap:Type) (a:Type) = st_post_h' heap a True
 let st_wp_h    (heap:Type) (a:Type) = st_post_h heap a -> Tot (st_pre_h heap)
 
@@ -34,7 +34,7 @@ unfold let st_bind_wp       (heap:Type)
                             (wp2:(a -> GTot (st_wp_h heap b)))
                             (p:st_post_h heap b) (h0:heap) =
   wp1 (fun a h1 -> wp2 a p h1) h0
-unfold let st_if_then_else  (heap:Type) (a:Type) (p:Type)
+unfold let st_if_then_else  (heap:Type) (a:Type) (p:prop)
                              (wp_then:st_wp_h heap a) (wp_else:st_wp_h heap a)
                              (post:st_post_h heap a) (h0:heap) =
      l_ITE p
@@ -54,11 +54,11 @@ unfold let st_close_wp      (heap:Type) (a:Type) (b:Type)
                              (wp:(b -> GTot (st_wp_h heap a)))
                              (p:st_post_h heap a) (h:heap) =
      (forall (b:b). wp b p h)
-unfold let st_assert_p      (heap:Type) (a:Type) (p:Type)
+unfold let st_assert_p      (heap:Type) (a:Type) (p:prop)
                              (wp:st_wp_h heap a)
                              (q:st_post_h heap a) (h:heap) =
      p /\ wp q h
-unfold let st_assume_p      (heap:Type) (a:Type) (p:Type)
+unfold let st_assume_p      (heap:Type) (a:Type) (p:prop)
                              (wp:st_wp_h heap a)
                              (q:st_post_h heap a) (h:heap) =
      p ==> wp q h
@@ -90,15 +90,15 @@ noeq type result (a:Type) =
   | Err : msg:string -> result a
 
 (* Effect EXCEPTION *)
-let ex_pre  = Type0
-let ex_post' (a:Type) (pre:Type) = (_:result a{pre}) -> GTot Type0
+let ex_pre  = prop
+let ex_post' (a:Type) (pre:Type) = (_:result a{pre}) -> GTot prop
 let ex_post  (a:Type) = ex_post' a True
 let ex_wp    (a:Type) = ex_post a -> GTot ex_pre
-unfold let ex_return   (a:Type) (x:a) (p:ex_post a) : GTot Type0 = p (V x)
+unfold let ex_return   (a:Type) (x:a) (p:ex_post a) : GTot prop = p (V x)
 unfold let ex_bind_wp (r1:range) (a:Type) (b:Type)
 		       (wp1:ex_wp a)
 		       (wp2:(a -> GTot (ex_wp b))) (p:ex_post b)
-         : GTot Type0 =
+         : GTot prop =
   forall (k:ex_post b).
      (forall (rb:result b).{:pattern (guard_free (k rb))} p rb ==> k rb)
      ==> (wp1 (function
@@ -111,7 +111,7 @@ unfold let ex_ite_wp (a:Type) (wp:ex_wp a) (post:ex_post a) =
      (forall (rb:result a).{:pattern (guard_free (k rb))} post rb ==> k rb)
      ==> wp k
 
-unfold let ex_if_then_else (a:Type) (p:Type) (wp_then:ex_wp a) (wp_else:ex_wp a) (post:ex_post a) =
+unfold let ex_if_then_else (a:Type) (p:prop) (wp_then:ex_wp a) (wp_else:ex_wp a) (post:ex_post a) =
    l_ITE p
        (wp_then post)
        (wp_else post)
@@ -119,8 +119,8 @@ unfold let ex_stronger (a:Type) (wp1:ex_wp a) (wp2:ex_wp a) =
         (forall (p:ex_post a). wp1 p ==> wp2 p)
 
 unfold let ex_close_wp (a:Type) (b:Type) (wp:(b -> GTot (ex_wp a))) (p:ex_post a) = (forall (b:b). wp b p)
-unfold let ex_assert_p (a:Type) (q:Type) (wp:ex_wp a) (p:ex_post a) = (q /\ wp p)
-unfold let ex_assume_p (a:Type) (q:Type) (wp:ex_wp a) (p:ex_post a) = (q ==> wp p)
+unfold let ex_assert_p (a:Type) (q:prop) (wp:ex_wp a) (p:ex_post a) = (q /\ wp p)
+unfold let ex_assume_p (a:Type) (q:prop) (wp:ex_wp a) (p:ex_post a) = (q ==> wp p)
 unfold let ex_null_wp (a:Type) (p:ex_post a) = (forall (r:result a). p r)
 unfold let ex_trivial (a:Type) (wp:ex_wp a) = wp (fun r -> True)
 
@@ -145,8 +145,8 @@ unfold let lift_div_exn (a:Type) (wp:pure_wp a) (p:ex_post a) = wp (fun a -> p (
 sub_effect DIV ~> EXN = lift_div_exn
 effect Ex (a:Type) = Exn a True (fun v -> True)
 
-let all_pre_h   (h:Type)           = h -> GTot Type0
-let all_post_h' (h:Type) (a:Type) (pre:Type)  = result a -> (_:h{pre}) -> GTot Type0
+let all_pre_h   (h:Type)           = h -> GTot prop
+let all_post_h' (h:Type) (a:Type) (pre:Type)  = result a -> (_:h{pre}) -> GTot prop
 let all_post_h  (h:Type) (a:Type)  = all_post_h' h a True
 let all_wp_h    (h:Type) (a:Type)  = all_post_h h a -> Tot (all_pre_h h)
 
@@ -160,13 +160,13 @@ unfold let all_return  (heap:Type) (a:Type) (x:a) (p:all_post_h heap a) = p (V x
 unfold let all_bind_wp (heap:Type) (r1:range) (a:Type) (b:Type)
                        (wp1:all_wp_h heap a)
                        (wp2:(a -> GTot (all_wp_h heap b)))
-                       (p:all_post_h heap b) (h0:heap) : GTot Type0 =
+                       (p:all_post_h heap b) (h0:heap) : GTot prop =
   wp1 (fun ra h1 -> (match ra with
                   | V v     -> wp2 v p h1
 		  | E e     -> p (E e) h1
 		  | Err msg -> p (Err msg) h1)) h0
 
-unfold let all_if_then_else (heap:Type) (a:Type) (p:Type)
+unfold let all_if_then_else (heap:Type) (a:Type) (p:prop)
                              (wp_then:all_wp_h heap a) (wp_else:all_wp_h heap a)
                              (post:all_post_h heap a) (h0:heap) =
    l_ITE p
@@ -180,10 +180,10 @@ unfold let all_close_wp (heap:Type) (a:Type) (b:Type)
                          (wp:(b -> GTot (all_wp_h heap a)))
                          (p:all_post_h heap a) (h:heap) =
     (forall (b:b). wp b p h)
-unfold let all_assert_p (heap:Type) (a:Type) (p:Type)
+unfold let all_assert_p (heap:Type) (a:Type) (p:prop)
                          (wp:all_wp_h heap a) (q:all_post_h heap a) (h:heap) =
     p /\ wp q h
-unfold let all_assume_p (heap:Type) (a:Type) (p:Type)
+unfold let all_assume_p (heap:Type) (a:Type) (p:prop)
                          (wp:all_wp_h heap a) (q:all_post_h heap a) (h:heap) =
     p ==> wp q h
 unfold let all_null_wp (heap:Type) (a:Type)
@@ -220,10 +220,11 @@ let allow_inversion (a:Type)
 //allowing inverting option without having to globally increase the fuel just for this
 val invertOption : a:Type -> Lemma
   (requires True)
-  (ensures (forall (x:option a). None? x \/ Some? x))
+  (ensures (forall (x:option a). b2p (None? x) \/ b2p (Some? x))) // TODO: drop b2p
   [SMTPat (option a)]
 let invertOption a = allow_inversion (option a)
 
+noeq // TODO
 type either 'a 'b =
   | Inl : v:'a -> either 'a 'b
   | Inr : v:'b -> either 'a 'b
@@ -237,6 +238,7 @@ val dsnd : #a:Type -> #b:(a -> GTot Type) -> t:dtuple2 a b -> Tot (b (Mkdtuple2?
 let dsnd #a #b t = Mkdtuple2?._2 t
 
 (* Concrete syntax (x:a & y:b x & c x y) *)
+noeq // TODO
 unopteq type dtuple3 (a:Type)
              (b:(a -> GTot Type))
              (c:(x:a -> b x -> GTot Type)) =
@@ -246,6 +248,7 @@ unopteq type dtuple3 (a:Type)
              -> dtuple3 a b c
 
 (* Concrete syntax (x:a & y:b x & z:c x y & d x y z) *)
+noeq // TODO
 unopteq type dtuple4 (a:Type)
              (b:(x:a -> GTot Type))
              (c:(x:a -> b x -> GTot Type))
@@ -259,7 +262,7 @@ unopteq type dtuple4 (a:Type)
 val ignore: #a:Type -> a -> Tot unit
 let ignore #a x = ()
 irreducible
-let rec false_elim (#a:Type) (u:unit{false}) : Tot a = false_elim ()
+let rec false_elim (#a:Type) (u:unit{False}) : Tot a = false_elim ()
 
 (* These are the supported attributes for top-level declarations. Syntax
  * example:
@@ -271,6 +274,7 @@ let rec false_elim (#a:Type) (u:unit{false}) : Tot a = false_elim ()
  * desugared but not type-checked; using the constructors of a data type
  * guarantees a minimal amount of typo-checking.
  * *)
+noeq // TODO
 type __internal_ocaml_attributes =
   | PpxDerivingShow
     (* Generate [@@ deriving show ] on the resulting OCaml type *)
